Prove tail-recursive pegexec function correct for PEGs+error-reporting

examples/formal-languages/context-free/pegexecScript.sml
@@ -13,13 +13,16 @@ Datatype:
     ksym (('atok,'bnt,'cvalue,'err) pegsym) kont kont
   | appf1 ('cvalue -> 'cvalue) kont
   | appf2 ('cvalue -> 'cvalue -> 'cvalue) kont
+  | dropErr kont
+  | addErr locs 'err kont
+  | cmpErrs kont
   | returnTo (('atok # locs) list) ('cvalue option list) kont
   | poplist ('cvalue list -> 'cvalue) kont
   | listsym (('atok,'bnt,'cvalue,'err) pegsym)
             ('cvalue list -> 'cvalue)
             kont
   | done
-  | failed locs 'err
+  | failed
 End
 
 val poplist_aux_def = Define`
@@ -36,11 +39,15 @@ val poplistval_def = Define`
 
 Datatype:
   evalcase = EV (('atok,'bnt,'cvalue,'err) pegsym)
-                (('atok # locs) list) ('cvalue option list)
+                (('atok # locs) list)
+                ('cvalue option list)
+                ((locs # 'err) list)
                 (('atok,'bnt,'cvalue,'err) kont)
                 (('atok,'bnt,'cvalue,'err) kont)
            | AP (('atok,'bnt,'cvalue,'err) kont)
-                (('atok # locs) list) ('cvalue option list)
+                (('atok # locs) list)
+                ('cvalue option list)
+                ((locs # 'err) list)
            | Result ((('atok # locs) list, 'cvalue, 'err) pegresult)
            | Looped
 End
@@ -50,63 +57,83 @@ Definition coreloop_def[nocompute]:
    OWHILE (λs. case s of Result _ => F
                        | _ => T)
           (λs. case s of
-                   EV (empty v) i r k fk => AP k i (SOME v::r)
-                 | EV (any tf) i r k fk =>
+                   EV (empty v) i r errs k fk => AP k i (SOME v::r) errs
+                 | EV (any tf) i r errs k fk =>
                    (case i of
-                        [] => AP fk i r
-                      | h::t => AP k t (SOME (tf h) :: r))
-                 | EV (tok P tf2) i r k fk =>
+                        [] => AP fk i r ((sloc i, G.anyEOF)::errs)
+                      | h::t => AP k t (SOME (tf h) :: r) errs)
+                 | EV (tok P tf2) i r errs k fk =>
                    (case i of
-                        [] => AP fk i r
-                      | h::t => if P (FST h) then AP k t (SOME (tf2 h)::r)
-                                else AP fk i r)
-                 | EV (nt n tf3) i r k fk =>
+                        [] => AP fk i r ((sloc i, G.tokEOF)::errs)
+                      | h::t => if P (FST h) then
+                                  AP k t (SOME (tf2 h)::r) errs
+                                else AP fk i r ((sloc i, G.tokFALSE)::errs))
+                 | EV (nt n tf3) i r errs k fk =>
                    if n ∈ FDOM G.rules then
-                     EV (G.rules ' n) i r (appf1 tf3 k) fk
+                     EV (G.rules ' n) i r errs (appf1 tf3 k) fk
                    else
                      Looped
-                 | EV (seq e1 e2 f) i r k fk =>
-                     EV e1 i r
+                 | EV (seq e1 e2 f) i r errs k fk =>
+                     EV e1 i r errs
                         (ksym e2 (appf2 f k) (returnTo i r fk))
                         fk
-                 | EV (choice e1 e2 cf) i r k fk =>
-                     EV e1 i r
+                 | EV (choice e1 e2 cf) i r errs k fk =>
+                     EV e1 i r errs
                         (appf1 (cf o INL) k)
-                        (returnTo i r (ksym e2 (appf1 (cf o INR) k) fk))
-                 | EV (rpt e lf) i r k fk =>
-                     EV e i (NONE::r) (listsym e lf k) (poplist lf k)
-                 | EV (not e v) i r k fk =>
-                     EV e i r (returnTo i r fk) (returnTo i (SOME v::r) k)
-                 | EV (error err) i r k fk => AP fk i r
-                 | AP done i [] => Looped
-                 | AP done i (NONE :: t) => Looped
-                 | AP done i (SOME rv :: _) => Result (Success i rv)
-                 | AP (failed l e) i r => Result (Failure l e)
-                 | AP (ksym e k fk) i r => EV e i r k fk
-                 | AP (appf1 f1 k) i (SOME v :: r) => AP k i (SOME (f1 v) :: r)
-                 | AP (appf1 _ _) _ _ => Looped
-                 | AP (appf2 f2 k) i (SOME v1 :: SOME v2 :: r) =>
-                     AP k i (SOME (f2 v2 v1) :: r)
-                 | AP (appf2 _ _) _ _ => Looped
-                 | AP (returnTo i r k) i' r' => AP k i r
-                 | AP (listsym e f k) i r =>
-                     EV e i r (listsym e f k) (poplist f k)
-                 | AP (poplist f k) i r => AP k i (poplistval f r)
+                        (returnTo i r
+                         (ksym e2
+                          (dropErr (appf1 (cf o INR) k))
+                          (cmpErrs fk)))
+                 | EV (rpt e lf) i r errs k fk =>
+                     EV e i (NONE::r) errs (listsym e lf k) (poplist lf k)
+                 | EV (not e v) i r errs k fk =>
+                     EV e i r errs
+                        (returnTo i r (addErr (sloc i) G.notFAIL fk))
+                        (returnTo i (SOME v::r) (dropErr k))
+                 | EV (error err) i r errs k fk =>
+                     AP fk i r ((sloc i, err) :: errs)
+                 | AP done i [] _ => Looped
+                 | AP done i (NONE :: t) _ => Looped
+                 | AP done i (SOME rv :: _) _ => Result (Success i rv)
+                 | AP failed i r [] => Looped
+                 | AP failed i r ((l,e)::_) => Result (Failure l e)
+                 | AP (dropErr _) i r [] => Looped
+                 | AP (dropErr k) i r (_ :: t) => AP k i r t
+                 | AP (addErr l e k) i r errs => AP k i r ((l,e)::errs)
+                 | AP (cmpErrs k) i r [] => Looped
+                 | AP (cmpErrs k) i r [_] => Looped
+                 | AP (cmpErrs k) i r ((l2,er2)::(l1,er1)::rest) =>
+                     AP k i r ((if locsle l1 l2 then (l2,er2) else (l1,er1)) ::
+                               rest)
+                 | AP (ksym e k fk) i r errs => EV e i r errs k fk
+                 | AP (appf1 f1 k) i (SOME v :: r) errs =>
+                     AP k i (SOME (f1 v) :: r) errs
+                 | AP (appf1 _ _) _ _ _ => Looped
+                 | AP (appf2 f2 k) i (SOME v1 :: SOME v2 :: r) errs =>
+                     AP k i (SOME (f2 v2 v1) :: r) errs
+                 | AP (appf2 _ _) _ _ _ => Looped
+                 | AP (returnTo i r k) i' r' errs => AP k i r errs
+                 | AP (listsym e f k) i r errs =>
+                     EV e i r errs (listsym e f k) (poplist f k)
+                 | AP (poplist f k) i r [] => Looped
+                 | AP (poplist f k) i r (_ :: errs) =>
+                     AP k i (poplistval f r) errs
                  | Result r => Result r
                  | Looped => Looped)
 End
 
 Definition peg_exec_def[nocompute]:
-  peg_exec (G:('atok,'bnt,'cvalue,'err)peg) e i r k fk =
-    case coreloop G (EV e i r k fk) of
+  peg_exec (G:('atok,'bnt,'cvalue,'err)peg) e i r errs k fk =
+    case coreloop G (EV e i r errs k fk) of
         SOME r => r
       | NONE => Looped
 End
 
 Definition applykont_def[nocompute]:
-  applykont G k i r = case coreloop G (AP k i r) of
-                          SOME r => r
-                        | NONE => Looped
+  applykont G k i r errs =
+  case coreloop G (AP k i r errs) of
+    SOME r => r
+  | NONE => Looped
 End
 
 Theorem coreloop_result[simp]:
@@ -157,15 +184,22 @@ val better_apply =
          ([`k` |-> `appf1 f k`, `r` |-> `SOME v::r`], []),
          ([`k` |-> `appf2 f k`, `r` |-> `SOME v1::SOME v2::r`], []),
          ([`k` |-> `returnTo i' r' k`], []),
+         ([‘k’ |-> ‘addErr l e k’], []),
+         ([‘k’ |-> ‘dropErr k’, ‘errs’ |-> ‘[]’], []),
+         ([‘k’ |-> ‘dropErr k’, ‘errs’ |-> ‘e::errs’], []),
+         ([‘k’ |-> ‘cmpErrs k’, ‘errs’ |-> ‘(l1,er1)::(l2,er2)::errs’], []),
          ([`k` |-> `done`, ‘r’ |-> ‘[]’], []),
          ([`k` |-> `done`, ‘r’ |-> ‘NONE::rs’], []),
          ([`k` |-> `done`, ‘r’ |-> ‘SOME rv::rs’], []),
-         ([`k` |-> `failed l e`], []),
-         ([`k` |-> `poplist f k`], []),
+         ([`k` |-> `failed`, ‘errs’ |-> ‘[]’], []),
+         ([`k` |-> `failed`, ‘errs’ |-> ‘(l,e)::errs’], []),
+         ([`k` |-> `poplist f k`, ‘errs’ |-> ‘[]’], []),
+         ([`k` |-> `poplist f k`, ‘errs’ |-> ‘le::errs’], []),
          ([`k` |-> `listsym e f k`], [])]
 
 Theorem peg_nt_thm =
   peg_exec_thm ([`e` |-> `nt n nfn`], [Once COND_RAND, option_case_COND])
+  |> SIMP_RULE (srw_ss()) []
 
 Theorem peg_exec_thm = LIST_CONJ better_peg_execs
 
@@ -177,31 +211,35 @@ val _ = app (fn s => ignore (remove_ovl_mapping s {Thy = "pegexec", Name = s}))
             ["AP", "EV"]
 
 Theorem exec_correct0[local]:
-  (∀i e r. peg_eval G (i,e) r ⇒
-           (∀j v k fk stk.
-              r = Success j v ⇒
-              peg_exec G e i stk k fk = applykont G k j (SOME v :: stk)) ∧
-           (∀k fk stk l err.
-              r = Failure l err ⇒
-              peg_exec G e i stk k fk = applykont G fk i stk)) ∧
+  (∀i e r.
+     peg_eval G (i,e) r ⇒
+     (∀j v k fk stk errs.
+        r = Success j v ⇒
+        peg_exec G e i stk errs k fk = applykont G k j (SOME v :: stk) errs) ∧
+     (∀k fk stk errs l err.
+        r = Failure l err ⇒
+        peg_exec G e i stk errs k fk = applykont G fk i stk ((l,err)::errs))) ∧
   (∀i e j vlist.
      peg_eval_list G (i,e) (j,vlist) ⇒
-     ∀f k stk vs.
+     ∀f k stk errs vs.
        peg_exec G e i (MAP SOME vs ++ (NONE::stk))
+                errs
                 (listsym e f k)
                 (poplist f k) =
-       applykont G k j (SOME (f (REVERSE vs ++ vlist)) :: stk))
+       applykont G k j (SOME (f (REVERSE vs ++ vlist)) :: stk) errs)
 Proof
   ho_match_mp_tac peg_eval_strongind' >>
   simp[peg_exec_thm, peg_nt_thm, applykont_thm, FORALL_result, AllCaseEqs()] >>
   rpt conj_tac
+  >- ((* locsle comparison *) rw[])
   >- ((* rpt - no elements succeed *)
       map_every qx_gen_tac [`e`, `f`, `i`, `j`, `vlist`] >> strip_tac >>
-      map_every qx_gen_tac [`k`, `stk`] >>
-      first_x_assum (qspecl_then [`f`, `k`, `stk`, `[]`] mp_tac) >>
+      map_every qx_gen_tac [`k`, `stk`, ‘errs’] >>
+      first_x_assum (qspecl_then [`f`, `k`, `stk`, ‘errs’, `[]`] mp_tac) >>
       simp[])
   >- ((* poplistval works *)
-      rpt strip_tac >> rpt AP_TERM_TAC >> rpt (pop_assum (K ALL_TAC)) >>
+      rpt strip_tac >> rpt (AP_TERM_TAC ORELSE AP_THM_TAC) >>
+      rpt (pop_assum (K ALL_TAC)) >>
       simp[poplistval_def] >>
       qmatch_abbrev_tac `
         (λ(values,rest). SOME (f values)::rest)
@@ -212,8 +250,8 @@ Proof
       Induct_on `vs` >> simp[poplist_aux_def])
   >- ((* rpt - some elements succeed *)
       map_every qx_gen_tac [`e`, `i0`, `i1`, `j`, `v`, `vs`] >> strip_tac >>
-      map_every qx_gen_tac [`f`, `k`, `stk`, `vs'`] >>
-      first_x_assum (qspecl_then [`f`, `k`, `stk`, `v::vs'`] mp_tac) >>
+      map_every qx_gen_tac [`f`, `k`, `stk`, ‘errs’, `vs'`] >>
+      first_x_assum (qspecl_then [`f`, `k`, `stk`, ‘errs’, `v::vs'`] mp_tac) >>
       simp[] >>
       simp_tac bool_ss [GSYM listTheory.APPEND_ASSOC, listTheory.APPEND])
 QED
@@ -224,13 +262,14 @@ Theorem exec_correct =
 Theorem pegexec_succeeds =
   exec_correct
     |> CONJUNCTS |> hd |> SPEC_ALL
-    |> Q.INST [`k` |-> `done`, `fk` |-> `failed l err`, `stk` |-> `[]`]
+    |> Q.INST [`k` |-> `done`, `fk` |-> `failed`, `stk` |-> `[]`,
+               ‘errs’ |-> ‘[]’]
     |> SIMP_RULE (srw_ss()) [applykont_thm]
 
 Theorem pegexec_fails =
   exec_correct |> CONJUNCTS |> tl |> hd |> SPEC_ALL
-               |> Q.INST [`k` |-> `done`, `fk` |-> `failed l err`,
-                          `stk` |-> `[]`]
+               |> Q.INST [`k` |-> `done`, `fk` |-> `failed`,
+                          `stk` |-> `[]`, ‘errs’ |-> ‘[]’]
                |> SIMP_RULE (srw_ss()) [applykont_thm]
 
 val pair_CASES = pairTheory.pair_CASES
@@ -238,78 +277,76 @@ val option_CASES = optionTheory.option_nchotomy
 val list_CASES = listTheory.list_CASES
 
 Theorem pegexec:
-  peg_eval G (s,e) r ⇒ peg_exec G e s [] done (failed l err) = Result r
+  peg_eval G (s,e) r ⇒ peg_exec G e s [] [] done failed = Result r
 Proof
-  metis_tac [option_CASES, pair_CASES, pegexec_fails, pegexec_succeeds]
+  strip_tac >>
+  Cases_on ‘r’ >> (drule pegexec_succeeds ORELSE drule pegexec_fails) >>
+  simp[]
 QED
 
-val peg_eval_executed = store_thm(
-  "peg_eval_executed",
-  ``wfG G ∧ e ∈ Gexprs G ⇒
-    (peg_eval G (s,e) r ⇔ peg_exec G e s [] done failed = Result r)``,
-  strip_tac >> eq_tac
-  >- (`r = NONE ∨ ∃s' v. r = SOME (s',v)`
-        by metis_tac[option_CASES, pair_CASES] >>
-      simp[pegexec_fails, pegexec_succeeds]) >>
+Theorem peg_eval_executed:
+  wfG G ∧ e ∈ Gexprs G ⇒
+    (peg_eval G (s,e) r ⇔ peg_exec G e s [] [] done failed = Result r)
+Proof
+  strip_tac >> eq_tac >- simp[pegexec] >>
   strip_tac >>
   `∃r'. peg_eval G (s,e) r'` by metis_tac[peg_eval_total] >>
   first_assum (assume_tac o MATCH_MP (CONJUNCT1 peg_deterministic)) >>
-  simp[] >> first_x_assum (assume_tac o MATCH_MP pegexec) >> fs[]);
+  simp[] >> first_x_assum (assume_tac o MATCH_MP pegexec) >> fs[]
+QED
 
-val destResult_def = Define`destResult (Result r) = r`
-val _ = export_rewrites ["destResult_def"]
+Definition destResult_def[simp]: destResult (Result r) = r
+End
 
-val pegparse_def = Define`
+Definition pegparse_def:
   pegparse G s =
-    if wfG G then destResult (peg_exec G G.start s [] done failed)
+    if wfG G then
+      case destResult (peg_exec G G.start s [] [] done failed) of
+        Success s v => SOME (s,v)
+      | _ => NONE
     else NONE
-`;
+End
 
-val pegparse_eq_SOME = store_thm(
-  "pegparse_eq_SOME",
-  ``pegparse G s = SOME (s',v) ⇔ wfG G ∧ peg_eval G (s,G.start) (SOME(s',v))``,
+Theorem pegparse_eq_SOME:
+  pegparse G s = SOME (s', v) ⇔
+  wfG G ∧ peg_eval G (s,G.start) (Success s' v)
+Proof
   Tactical.REVERSE (Cases_on `wfG G`) >- simp[pegparse_def] >>
   `∃r. peg_eval G (s,G.start) r`
     by metis_tac [peg_eval_total, start_IN_Gexprs] >>
   first_assum (assume_tac o MATCH_MP (CONJUNCT1 peg_deterministic)) >>
   simp[] >>
-  `r = NONE ∨ ∃s2 v2. r = SOME (s2,v2)` by metis_tac [option_CASES, pair_CASES]
-  >- rw[pegparse_def, pegexec_fails] >>
-  rw[pegparse_def] >> first_x_assum (assume_tac o MATCH_MP pegexec_succeeds) >>
-  simp[] >> metis_tac[]);
+  reverse (Cases_on ‘r’)
+  >- (rw[pegparse_def] >> drule pegexec_fails >> simp[]) >>
+  rw[pegparse_def] >> drule pegexec_succeeds >> simp[] >> metis_tac[]
+QED
 
-val pegparse_eq_NONE = store_thm(
-  "pegparse_eq_NONE",
-  ``pegparse G s = NONE ⇔ ¬wfG G ∨ peg_eval G (s,G.start) NONE``,
+Theorem pegparse_eq_NONE:
+  pegparse G s = NONE ⇔ ¬wfG G ∨ ∃l e. peg_eval G (s,G.start) (Failure l e)
+Proof
   Cases_on `wfG G` >> simp[pegparse_def] >>
   `∃r. peg_eval G (s,G.start) r`
     by metis_tac [peg_eval_total, start_IN_Gexprs] >>
   first_assum (assume_tac o MATCH_MP (CONJUNCT1 peg_deterministic)) >>
-  simp[] >>
-  `r = NONE ∨ ∃s2 v2. r = SOME (s2,v2)` by metis_tac [option_CASES, pair_CASES]
-  >- rw[pegexec_fails] >>
-  rw[] >> first_x_assum (assume_tac o MATCH_MP pegexec_succeeds) >>
-  simp[]);
+  simp[] >> reverse (Cases_on ‘r’) >> simp[]
+  >- (drule pegexec_fails >> simp[]) >>
+  drule pegexec_succeeds >> simp[]
+QED
 
-val peg_exec_total = store_thm(
-  "peg_exec_total",
-  ``wfG G ==> ∃r. peg_exec G G.start i [] done failed = Result r``,
+Theorem peg_exec_total:
+  wfG G ==> ∃r. peg_exec G G.start i [] [] done failed = Result r
+Proof
   strip_tac >>
   `∃pr. peg_eval G (i, G.start) pr` by simp[peg_eval_total, start_IN_Gexprs] >>
-  pop_assum mp_tac >> simp[peg_eval_executed, start_IN_Gexprs]);
-
-val option_case_EQ = prove(
-  ``option_CASE x n s = v ⇔ x = NONE ∧ n = v ∨ ∃v0. x = SOME v0 ∧ v = s v0``,
-  Cases_on `x` >> simp[] >> metis_tac[]);
+  pop_assum mp_tac >> simp[peg_eval_executed, start_IN_Gexprs]
+QED
 
 (*
    |- wfG G ⇒
       ∃r.
         coreloop G (pegexec$EV G.start i [] done failed) = SOME (Result r)
 *)
-val coreloop_total = save_thm(
-  "coreloop_total",
-  peg_exec_total |> SIMP_RULE (srw_ss()) [peg_exec_def, option_case_EQ])
-
+Theorem coreloop_total =
+  peg_exec_total |> SIMP_RULE (srw_ss()) [peg_exec_def, AllCaseEqs()]
 
 val _ = export_theory()
